Carpetas y nuevas funciones

src/Knapsack/Specification/SolutionData.dfy
@@ -1,19 +1,7 @@
-include "ContainersOps.dfy"
-include "Math.dfy"
-//A nivel de especificación tenemos estos datatype
-
-datatype ItemData = ItemData(weight: real, value: real) {
-  ghost predicate Valid() {
-    weight > 0.0 && value > 0.0
-  }
-}
-
-datatype InputData = InputData(items: seq<ItemData>, maxWeight: real) {
-  ghost predicate Valid() {
-    (forall i | 0 <= i < |items| :: items[i].Valid()) &&
-    maxWeight >= 0.0
-  }
-}
+include "InputData.dfy"
+include "ItemData.dfy"
+include "../../ContainersOps.dfy"
+include "../../Math.dfy"
 
 datatype SolutionData = SolutionData(itemsAssign: seq<bool>, k: nat) {
 
@@ -27,7 +15,7 @@ datatype SolutionData = SolutionData(itemsAssign: seq<bool>, k: nat) {
     sum_real(weightsSelected, 0, numSelected)
   }
 
-  ghost function Value(items: seq<ItemData>): (o: real)
+  ghost function TotalValue(items: seq<ItemData>): (o: real)
     requires k <= |items|
     requires k <= |itemsAssign|
   {
@@ -37,17 +25,25 @@ datatype SolutionData = SolutionData(itemsAssign: seq<bool>, k: nat) {
     sum_real(valuesSelected, 0, numSelected)
   }
 
+  ghost predicate Partial (input: InputData){
+    && 0 <= k <= |itemsAssign| 
+    && |itemsAssign| == |input.items|
+    && this.TotalWeight(input.items) <= input.maxWeight
+  }
+
+  ghost predicate Valid(input: InputData){
+    && 0 <= k <= |itemsAssign| 
+    && |itemsAssign| == |input.items|
+    && this.TotalWeight(input.items) <= input.maxWeight
+  }
+
   ghost predicate Optimal(input: InputData)
     requires this.Valid(input)
     requires input.Valid()
   {
-    forall otherSolution: SolutionData | otherSolution.Valid(input) :: otherSolution.Value(input.items) <= Value(input.items)
+    forall otherSolution: SolutionData | otherSolution.Valid(input) :: otherSolution.TotalValue(input.items) <= TotalValue(input.items)
   }
 
-  ghost predicate Valid(input: InputData){
-    0 <= k <= |itemsAssign| &&
-    |itemsAssign| == |input.items|
-    && this.TotalWeight(input.items) <= input.maxWeight
-  }
-
+  
+  
 }
