src/Knapsack/Specification/InputData.dfy
@@ -1,0 +1,8 @@
+include "ItemData.dfy"
+
+datatype InputData = InputData(items: seq<ItemData>, maxWeight: real) {
+  ghost predicate Valid() {
+    (forall i | 0 <= i < |items| :: items[i].Valid()) &&
+    maxWeight >= 0.0
+  }
+}
