src/Knapsack/Specification/ItemData.dfy
@@ -1,0 +1,6 @@
+
+datatype ItemData = ItemData(weight: real, value: real) {
+  ghost predicate Valid() {
+    weight > 0.0 && value > 0.0
+  }
+}
